Demo: progress in safety in C module

rustdemo/HashMapSafe.v
@@ -5,11 +5,11 @@ Require Import Integers.
 Require Import Floats.
 Require Import Values.
 Require Import AST.
-Require Import Cop Ctypes.
+Require Import Cop Ctypes Ctypesdefs.
 Require Import Values Globalenvs Memory.
 Require Import Events.
 Require Import Invariant Smallstep SmallstepLinkingSafe.
-Require Import Clight HashMap LinkedList.
+Require Import Clight HashMap LinkedList HashMapCommon.
 Require Import Separation.
 Require Import MoveCheckingFootprint MoveCheckingDomain.
 
@@ -17,15 +17,58 @@ Local Open Scope error_monad_scope.
 Local Open Scope sep_scope.
 Import ListNotations.
 
+Fixpoint num_frames_cont (k: cont) : nat :=
+  match k with
+  | Kstop => O
+  | Kcall _ _ _ _ k' =>
+      S (num_frames_cont k')
+  | Kseq _ k
+  | Kloop1 _ _ k
+  | Kloop2 _ _ k
+  | Kswitch k => num_frames_cont k
+  end.
+
+Definition num_frames (s: state) : nat :=
+  match s with
+  | State _ _ k _ _ _
+  | Callstate _ _ k _
+  | Returnstate _ k _ => num_frames_cont k
+  end.
+
+
 Definition hash_map_sem := semantics1 hash_map_prog.
+
+Definition int_to_nat (i: int) : nat :=
+  Z.to_nat (Int.unsigned i).
+
+Definition nat_to_int (n: nat) : int :=
+  Int.repr (Z.of_nat n).
+
 
 Section SOUNDNESS.
 
 Variable N : nat.
 
 Context (se : Genv.symtbl).
+Context (w: hmap_world).
 
 Let ge := globalenv se hash_map_prog.
+
+Let Ni := nat_to_int N.
+
+Hypothesis Neq10: N = 10%nat.
+
+Lemma Nieq : Ni = Int.repr 10.
+Proof.
+  unfold Ni. rewrite Neq10.
+  reflexivity.
+Qed.
+
+(** Combine it with the wf_senv in LinkedListSafe *)
+Hypothesis wf_senv: forall id,
+    if in_dec ident_eq id (prog_defs_names hash_map_prog) then
+      exists b, Genv.find_symbol se id = Some b
+    else True.
 
 Remark hmap_ce: genv_cenv ge = PTree.empty composite.
   reflexivity. Qed.
@@ -74,5 +117,397 @@ a more dedicated condition that distinguish the call to
 hmap_operate_on or process and then use different conditions. *)
 
 
+(* state invariant *)
+
+Definition return_find_bucket_cont k :=
+  (Kseq
+     (Sifthenelse
+        (Ebinop Oeq (Ederef (Evar buk List_box_ptr) List_ptr)
+           (Ecast (Econst_long (Int64.repr 0) tlong) (tptr tvoid)) tint) 
+        (Sreturn None)
+        (Ssequence
+           (Scall (Some tmp)
+              (Evar find
+                 (Tfunction (Tcons List_ptr (Tcons tint Tnil)) List_ptr cc_default))
+              [Ederef (Evar buk List_box_ptr) List_ptr; Evar key tint])
+           (Sassign (Ederef (Evar buk List_box_ptr) List_ptr) (Evar tmp List_ptr)))) k).
+
+(* The continuation (that inside Kcall) of calling find_bucket. The
+caller can be hmap_operate_on, hmap_set, hmap_remove. It outputs a
+predicate which describe the contents of hmap_operate_on. [b] is the
+block storing the hash_map *)
+Inductive call_find_bucket_from_operate_on (b: block) : cont -> massert -> Prop :=
+| call_find_bucket_from_operate_on_intro: forall k e le b_hmap b_key ki
+    (ENV: e = PTree.set key (b_key, tint) (PTree.set hmap (b_hmap, hmap_ty) empty_env))
+    (LENV: le = create_undef_temps (fn_temps hmap_operate_on_func)),
+    call_find_bucket_from_operate_on b (Kcall (Some buk) hmap_operate_on_func e le (return_find_bucket_cont k))
+                                     (contains Mptr b_hmap 0 (eq (Vptr b Ptrofs.zero))
+                                        ** contains Mint32 b_key 0 (eq (Vint ki)))
+.
+
+Inductive call_find_bucket_cont (b: block) : cont -> massert -> Prop :=
+(* from hmap_operate_on *)
+| call_find_bucket_cont_intro1: forall k MP
+    (CONT: call_find_bucket_from_operate_on b k MP),
+    call_find_bucket_cont b k MP
+(* TODO: from hmap_set *)
+.
+
+(* TODO *)
+Inductive call_hash_cont : cont -> Prop :=
+| call_hash_cont_intro: forall k,
+    call_hash_cont k.
+
+Inductive call_hmap_operate_on: state -> Prop :=
+| call_hmap_operate_on_intro: forall b1 b2 kv k m fpl
+    (SYM: Genv.invert_symbol se b1 = Some hmap_operate_on)
+    (** TODO: specify the cont *)
+    (HMAP: m |= hmap_pred b2 fpl),
+    call_hmap_operate_on (Callstate (Vptr b1 Ptrofs.zero) [Vptr b2 Ptrofs.zero; Vint kv] k m).
+
+Inductive call_find_bucket: state -> Prop :=
+| call_find_bucket_intro: forall b1 b2 kv k m fpl MP
+    (SYM: Genv.invert_symbol se b1 = Some find_bucket)
+    (CONT: call_find_bucket_cont b2 k MP)
+    (* MP is the predicate for the stack frames *)
+    (HMAP: m |= hmap_pred b2 fpl ** MP),
+    call_find_bucket (Callstate (Vptr b1 Ptrofs.zero) [Vptr b2 Ptrofs.zero; Vint kv] k m).
+ 
+
+Inductive sound_state : state -> Prop :=
+| hmap_operate_on_callstate: forall b1 b2 kv k m
+    (CALL: call_hmap_operate_on (Callstate (Vptr b1 Ptrofs.zero) [Vptr b2 Ptrofs.zero; Vint kv] k m)),
+    sound_state (Callstate (Vptr b1 Ptrofs.zero) [Vptr b2 Ptrofs.zero; Vint kv] k m)
+| hmap_operate_on_internal1: forall t s b_hmap b_key fpl ki b m e le k n
+    (MPRED: m |= contains Mptr b_hmap 0 (eq (Vptr b Ptrofs.zero))
+              ** contains Mint32 b_key 0 (eq (Vint ki))
+              ** hmap_pred b fpl)
+    (ENV: e = PTree.set key (b_key, tint) (PTree.set hmap (b_hmap, hmap_ty) empty_env))
+    (LENV: le = create_undef_temps (fn_temps hmap_operate_on_func))
+    (STAR: starNf step1 num_frames ge n (State hmap_operate_on_func (fn_body hmap_operate_on_func) k e le m) t s)
+    (RAN: (0<= n <=1)%nat),
+    sound_state s
+(* return from find_bucket *)
+| hmap_operate_on_internal2: forall t1 t2 s1 s2 n idx fpl1 fpl2 b fp m ofs k MP
+    (STEP: step1 ge (Returnstate (Vptr b ofs) k m) t1 s1)
+    (OFSEQ: ofs = (Ptrofs.mul (Ptrofs.repr (size_chunk Mptr)) (Ptrofs.of_int idx)))
+    (STAR: starNf step1 num_frames ge n s1 t2 s2)
+    (MPRED: m |= contains Mptr b (-size_chunk Mptr) (eq (Vptrofs (Ptrofs.repr (Z_of_nat N * size_chunk Mptr))))
+              ** hmap_pred_rec (int_to_nat idx) fpl1 b 0
+              ** bucket_pred b (Ptrofs.unsigned ofs) fp
+              ** hmap_pred_rec (N - 1 - (int_to_nat idx))%nat fpl2 b (Ptrofs.unsigned ofs + size_chunk Mptr)
+              ** MP)
+    (RAN: (0 <= n <= 10)%nat)
+    (CONT: call_find_bucket_from_operate_on b k MP),
+    sound_state s2
+| hmap_operate_on_returnstate: forall k m,
+    (** TODO: specify the cont *)
+    sound_state (Returnstate Vundef k m)
+| find_bucket_callstate: forall b1 b2 kv k m
+    (CALL: call_find_bucket (Callstate (Vptr b1 Ptrofs.zero) [Vptr b2 Ptrofs.zero; Vint kv] k m)),
+    sound_state (Callstate (Vptr b1 Ptrofs.zero) [Vptr b2 Ptrofs.zero; Vint kv] k m)
+| find_bucket_internal1: forall s0 t s n b_key b_hmap m k b fpl ki
+    (SEQ: s0 = (State find_bucket_func (fn_body find_bucket_func) k
+                  (PTree.set key (b_key, tint) (PTree.set hmap (b_hmap, hmap_ty) empty_env))
+                  (create_undef_temps (fn_temps find_bucket_func)) m))
+    (MPRED: m |= contains Mptr b_hmap 0 (eq (Vptr b Ptrofs.zero))
+              ** contains Mint32 b_key 0 (eq (Vint ki))
+              ** hmap_pred b fpl)
+    (STAR: starNf step1 num_frames ge n s0 t s)
+    (RAN: (0 <= n <= 1)%nat),
+    sound_state s
+(* at_external state calling hash function in the Rust side *)
+| find_bucket_call_hash: forall ki b k m
+    (COND: hash_pre_cond_args Ni [Vint ki; Vint Ni])
+    (FINDF: Genv.find_funct ge (Vptr b Ptrofs.zero) = Some hash_ext)
+    (** TODO: specify the continuation *)
+    (CONT: call_hash_cont k),
+    sound_state (Callstate (Vptr b Ptrofs.zero) [Vint ki; Vint Ni] k m)
+| find_bucket_return_hash: forall v k m
+    (COND: hash_post_cond_retv Ni v)
+    (CONT: call_hash_cont k),
+    sound_state (Returnstate v k m)
+| find_bucket_returnstate: forall idx fpl1 fpl2 b fp m ofs k MP
+    (OFSEQ: ofs = (Ptrofs.mul (Ptrofs.repr (size_chunk Mptr)) (Ptrofs.of_int idx)))
+    (MPRED: m |= contains Mptr b (-size_chunk Mptr) (eq (Vptrofs (Ptrofs.repr (Z_of_nat N * size_chunk Mptr))))
+              ** hmap_pred_rec (int_to_nat idx) fpl1 b 0
+              ** bucket_pred b (Ptrofs.unsigned ofs) fp
+              ** hmap_pred_rec (N - 1 - (int_to_nat idx))%nat fpl2 b (Ptrofs.unsigned ofs + size_chunk Mptr)
+              ** MP)
+    (CONT: call_find_bucket_cont b k MP),
+    sound_state (Returnstate (Vptr b ofs) k m)
+.
+
+
+Lemma function_entry1_det: forall ge f vl m m1 m2 e1 le1 e2 le2,
+    function_entry1 ge f vl m e1 le1 m1 ->
+    function_entry1 ge f vl m e2 le2 m2 ->
+    e1 = e2 /\ le1 = le2 /\ m1 = m2.
+Admitted.
+
+(* maybe we can have a general function_entry_rule *)
+Lemma function_entry_hmap_operate_on: forall m P b ofs ki,
+    m |= P ->
+    exists b1 b2 m', 
+      function_entry1 ge hmap_operate_on_func [Vptr b ofs; Vint ki] m (PTree.set key (b2, tint) (PTree.set hmap (b1, hmap_ty) empty_env)) (create_undef_temps (fn_temps hmap_operate_on_func)) m'
+      /\ m' |= contains Mptr b1 0 (eq (Vptr b ofs))
+          ** contains Mint32 b2 0 (eq (Vint ki))
+          ** P.
+Proof.
+  intros until ki. intros MP.
+  destruct (Mem.alloc m 0 (size_chunk Mptr)) eqn: ALLOC1.
+  destruct (Mem.alloc m0 0 (size_chunk Mint32)) eqn: ALLOC2.
+  exploit alloc_rule. eapply ALLOC1. lia. vm_compute. congruence.
+  eapply MP. intros MP1.
+  exploit alloc_rule. eapply ALLOC2. lia. vm_compute. congruence.
+  eapply MP1. intros MP2.
+  eapply sep_swap12 in MP2.
+  exploit storev_rule. eapply range_contains with (ofs:=0) (chunk:= Mptr). eauto.
+  eapply Z.divide_0_r.
+  instantiate (1 := Vptr b ofs). instantiate (1 := eq (Vptr b ofs)). auto.
+  intros (m2 & STORE1 & MP3).
+  eapply sep_swap12 in MP3.
+  exploit storev_rule. eapply range_contains with (ofs:=0) (chunk:= Mint32). eauto.
+  eapply Z.divide_0_r.
+  instantiate (1 := Vint ki). instantiate (1 := eq (Vint ki)). auto.
+  intros (m3 & STORE2 & MP4).
+  eapply sep_swap12 in MP4.
+  exists p, p0, m3. split.
+  econstructor.
+  eapply proj_sumbool_true with (a:= list_norepet_dec ident_eq [hmap; key]); eauto.
+  econstructor; eauto.
+  econstructor; eauto. econstructor.
+  econstructor. reflexivity.
+  econstructor. reflexivity. eauto.
+  econstructor. reflexivity.
+  econstructor. reflexivity. eauto.
+  econstructor. reflexivity.
+  auto.
+Qed.  
+
+(* The same as hmap_opearate_on because they have the same types of arguments *)
+Lemma function_entry_find_bucket: forall m P b ofs ki,
+    m |= P ->
+    exists b1 b2 m', 
+      function_entry1 ge find_bucket_func [Vptr b ofs; Vint ki] m (PTree.set key (b2, tint) (PTree.set hmap (b1, hmap_ty) empty_env)) (create_undef_temps (fn_temps find_bucket_func)) m'
+      /\ m' |= contains Mptr b1 0 (eq (Vptr b ofs))
+          ** contains Mint32 b2 0 (eq (Vint ki))
+          ** P.
+Proof.
+  intros until ki. intros MP.
+  destruct (Mem.alloc m 0 (size_chunk Mptr)) eqn: ALLOC1.
+  destruct (Mem.alloc m0 0 (size_chunk Mint32)) eqn: ALLOC2.
+  exploit alloc_rule. eapply ALLOC1. lia. vm_compute. congruence.
+  eapply MP. intros MP1.
+  exploit alloc_rule. eapply ALLOC2. lia. vm_compute. congruence.
+  eapply MP1. intros MP2.
+  eapply sep_swap12 in MP2.
+  exploit storev_rule. eapply range_contains with (ofs:=0) (chunk:= Mptr). eauto.
+  eapply Z.divide_0_r.
+  instantiate (1 := Vptr b ofs). instantiate (1 := eq (Vptr b ofs)). auto.
+  intros (m2 & STORE1 & MP3).
+  eapply sep_swap12 in MP3.
+  exploit storev_rule. eapply range_contains with (ofs:=0) (chunk:= Mint32). eauto.
+  eapply Z.divide_0_r.
+  instantiate (1 := Vint ki). instantiate (1 := eq (Vint ki)). auto.
+  intros (m3 & STORE2 & MP4).
+  eapply sep_swap12 in MP4.
+  exists p, p0, m3. split.
+  econstructor.
+  eapply proj_sumbool_true with (a:= list_norepet_dec ident_eq [hmap; key]); eauto.
+  econstructor; eauto.
+  econstructor; eauto. econstructor.
+  econstructor. reflexivity.
+  econstructor. reflexivity. eauto.
+  econstructor. reflexivity.
+  econstructor. reflexivity. eauto.
+  econstructor. reflexivity.
+  auto.
+Qed.  
+
+
+  
+Lemma step_preservation_progress: forall s,
+    sound_state s ->
+    not_stuck (hash_map_sem se) s
+    /\ (forall s' t, step1 ge s t s' ->
+               sound_state s').
+Proof.
+  intros s INV. inv INV.
+  (* call hmap_operate_on *)
+  - inv CALL.
+    assert (FIND: Genv.find_funct ge (Vptr b1 Ptrofs.zero) = Some (Internal hmap_operate_on_func)).
+    { simpl. destruct Ptrofs.eq_dec; try congruence.
+      eapply Genv.find_funct_ptr_iff.
+      rewrite Genv.find_def_spec. rewrite SYM.
+      auto. }
+    exploit (function_entry_hmap_operate_on m (hmap_pred b2 fpl) b2 Ptrofs.zero kv). eapply HMAP.
+    intros (b_hmap & b_key & m1 & ENTRY & MPRED1).
+    split.
+    + red. do 2 right.      
+      do 2 eexists. econstructor; eauto.
+    + intros. inv H; rewrite FIND in FIND0; inv FIND0.
+      exploit function_entry1_det. eauto. eapply ENTRY.
+      intros (A1 & A2 & A3). subst.
+      eapply hmap_operate_on_internal1. eauto.
+      reflexivity. reflexivity. econstructor. lia.
+  (* hmap_operate_on_internal1 *)
+  - generalize MPRED as MPRED1. intros.
+    generalize STAR as STAR1. intros.
+    inv STAR.
+    { split.
+      - red. do 2 right.
+        do 2 eexists. econstructor.
+      - intros. eapply hmap_operate_on_internal1 with (n:=1%nat); eauto.
+        eapply starNf_step_right; eauto. 
+        inv H; simpl; auto. }
+    inv STEP.
+    2: { destruct H7; try congruence. }
+    2: { destruct H7; try congruence. }
+    inv STAR0; cbn [num_frames num_frames_cont] in *.
+    { generalize (wf_senv find_bucket). intros FINDF.
+      simpl in FINDF. destruct FINDF as (?b & FINDF).
+      exploit load_rule. eapply sep_proj1. eapply MPRED.
+      intros (v1 & LOAD1 & SPEC1). subst.
+      exploit load_rule. eapply sep_proj1. eapply sep_proj2. eapply MPRED.
+      intros (v2 & LOAD2 & SPEC2). subst.
+      split.
+      - red. do 2 right.
+        do 2 eexists. econstructor.
+        reflexivity.
+        econstructor. eapply eval_Evar_global. reflexivity. eauto.
+        eapply deref_loc_reference. reflexivity.
+        econstructor. econstructor. eapply eval_Evar_local.
+        reflexivity. econstructor. reflexivity. eauto.
+        reflexivity.
+        econstructor. econstructor. eapply eval_Evar_local.
+        reflexivity. econstructor. reflexivity. eauto.
+        reflexivity.
+        econstructor.
+        (* find_funct *)
+        simpl. rewrite dec_eq_true. unfold Genv.find_funct_ptr.
+        rewrite Genv.find_def_spec.
+        erewrite Genv.find_invert_symbol; eauto.
+        reflexivity. reflexivity.
+      - intros. inv H.
+        simpl in H10. inv H10.
+        inv H12. inv H3. inv H.
+        2: { vm_compute in H3. congruence. }
+        vm_compute in H8. inv H8. inv H0; simpl in H; inv H. 
+        setoid_rewrite LOAD1 in H1. inv H1.
+        vm_compute in H5. inv H5.
+        inv H6. inv H3. inv H.
+        2: { vm_compute in H3. congruence. }
+        vm_compute in H8. inv H8. inv H0; simpl in H; inv H. 
+        setoid_rewrite LOAD2 in H1. inv H1.
+        vm_compute in H5. inv H5. inv H7.
+        exploit Genv.find_funct_inv. eauto.
+        intros (b1 & A1). subst.
+        inv H11. inv H.
+        vm_compute in H6. congruence.
+        inv H0. simpl in H; inv H.
+        2: { simpl in H1. inv H1. }
+        simpl in H7.
+        rewrite FINDF in H7. inv H7.
+        eapply find_bucket_callstate; eauto.
+        econstructor.
+        eapply Genv.find_invert_symbol. eauto.
+        (* cont *)
+        econstructor. econstructor. reflexivity.
+        reflexivity.
+        eapply sep_comm. rewrite sep_assoc.
+        eapply MPRED1. } 
+    lia.
+  (** TODO: hmap_operate_on after returning from find_bucket *)
+  - admit.
+  (* return from hmap_operate_on *)
+  - admit.
+  (* call find_bucket *)
+  - inv CALL. 
+    assert (FIND: Genv.find_funct ge (Vptr b1 Ptrofs.zero) = Some (Internal find_bucket_func)).
+    { simpl. destruct Ptrofs.eq_dec; try congruence.
+      eapply Genv.find_funct_ptr_iff.
+      rewrite Genv.find_def_spec. rewrite SYM.
+      auto. }    
+    exploit (function_entry_find_bucket m (hmap_pred b2 fpl) b2 Ptrofs.zero kv). eapply HMAP.    
+    intros (b_hmap & b_key & m1 & ENTRY & MPRED1).
+    split.
+    + red. do 2 right.      
+      do 2 eexists. econstructor; eauto.
+    + intros. inv H; rewrite FIND in FIND0; inv FIND0.
+      exploit function_entry1_det. eauto. eapply ENTRY.
+      intros (A1 & A2 & A3). subst.
+      eapply find_bucket_internal1 with (n:=0%nat). reflexivity. eauto.
+      econstructor. lia.
+  (* find_bucket_internal1  *)
+  - generalize MPRED as MPRED1. intros.
+    generalize STAR as STAR1. intros.
+    inv STAR.
+    { split.
+      - red. do 2 right.
+        do 2 eexists. econstructor.
+      - intros. eapply find_bucket_internal1 with (n:=1%nat); eauto.
+        eapply starNf_step_right; eauto. 
+        inv H; simpl; auto. }
+    inv STEP.
+    2: { destruct H7; try congruence. }
+    2: { destruct H7; try congruence. }
+    inv STAR0; cbn [num_frames num_frames_cont] in *.
+    { generalize (wf_senv hash). intros FINDF.
+      simpl in FINDF. destruct FINDF as (?b & FINDF).
+      exploit load_rule. eapply sep_proj1. eapply sep_proj2. eapply MPRED.
+      intros (v1 & LOAD1 & SPEC1). subst.
+      split.
+      - red. do 2 right.
+        do 2 eexists. econstructor.
+        reflexivity.
+        econstructor. eapply eval_Evar_global. reflexivity. eauto.
+        eapply deref_loc_reference. reflexivity.
+        econstructor. econstructor. eapply eval_Evar_local.
+        reflexivity. econstructor. reflexivity. eauto.
+        reflexivity.
+        econstructor. econstructor. 
+        reflexivity. econstructor. 
+        (* find_funct *)
+        simpl. rewrite dec_eq_true. unfold Genv.find_funct_ptr.
+        rewrite Genv.find_def_spec.
+        erewrite Genv.find_invert_symbol; eauto.
+        reflexivity. reflexivity.
+      - intros. inv H.
+        simpl in H10. inv H10.
+        inv H12. inv H3. inv H.
+        2: { vm_compute in H3. congruence. }
+        vm_compute in H8. inv H8. inv H0; simpl in H; inv H. 
+        setoid_rewrite LOAD1 in H1. inv H1. vm_compute in H5. inv H5.
+        inv H6. inv H3.
+        2: { inv H. }
+        erewrite cast_val_casted in H5.
+        2: { econstructor. reflexivity. }
+        inv H5.
+        exploit Genv.find_funct_inv. eauto.
+        intros (b1 & A1). subst.
+        inv H11. inv H.
+        vm_compute in H6. congruence.
+        inv H0. simpl in H; inv H.
+        2: { simpl in H1. inv H1. }
+        inv H7. simpl in H8.
+        replace (Int.repr 10) with Ni.
+        2: { unfold Ni. rewrite Neq10. reflexivity. }
+        eapply find_bucket_call_hash; eauto.
+        econstructor. rewrite Nieq. auto.
+        econstructor. reflexivity.
+        econstructor. reflexivity.
+        (* find_funct *)
+        simpl. rewrite dec_eq_true. unfold Genv.find_funct_ptr.
+        rewrite Genv.find_def_spec.
+        erewrite Genv.find_invert_symbol; eauto.
+        reflexivity. 
+        (* cont *)
+        econstructor.  }
+    lia.
+  (* call hash function *)
+  - admit.
+  Admitted.
+      
 End SOUNDNESS.
 
