rustdemo/HashMapCommon.v
@@ -1,0 +1,134 @@
+Require Import Coqlib.
+Require Import Errors.
+Require Import Maps.
+Require Import Integers.
+Require Import Floats.
+Require Import Values.
+Require Import AST.
+Require Import Cop Ctypes.
+Require Import Values Globalenvs Memory.
+Require Import Events.
+Require Import Invariant Smallstep SmallstepLinkingSafe.
+Require Import HashMap.
+Require Import LinkedList RustOp Rusttypes Rustlight Rustlightown.
+
+Local Open Scope error_monad_scope.
+Import ListNotations.
+
+
+Section CLOSURES.
+
+Context {genv: Type}.
+Context {state: Type}.
+
+Variable step: genv -> state -> trace -> state -> Prop.
+Variable numf: state -> nat.
+
+Inductive starNf (ge: genv): nat -> state -> trace -> state -> Prop :=
+  | starNf_refl: forall s,
+      starNf ge O s E0 s
+  | starNf_step: forall n s t t1 s' t2 s''
+      (STEP: step ge s t1 s')
+      (STAR: starNf ge n s' t2 s'')
+      (TRACE: t = t1 ** t2)
+      (FEQ: numf s = numf s'),
+      starNf ge (S n) s t s''.
+
+Remark starNf_star:
+  forall ge n s t s', starNf ge n s t s' -> star step ge s t s'.
+Proof.
+  induction 1; econstructor; eauto.
+Qed.
+
+Remark starNf_step_right ge: forall n s t t1 s' t2 s'',
+    starNf ge n s t1 s' -> step ge s' t2 s'' -> t = t1 ** t2 ->
+    numf s' = numf s'' ->
+    starNf ge (S n) s t s''.
+Admitted.
+
+End CLOSURES.
+
+
+(* The kripke world used in proving partial safety *)
+Record hmap_world :=
+  { 
+    hmap_callee: ident + ident;         (* remember the called
+    function (inl is in linked_list and inr is in the C module) to
+    specify the post condition when returning the current module. How
+    to generalize it? *)
+    hmap_senv: Genv.symtbl;
+    hmap_hash_range : int }.
+
+
+(* pre-post conditions of hash function *)
+
+Inductive hash_pre_cond_args r : list Values.val -> Prop :=
+| hash_pre_cond_args_intro: forall k
+    (GTZ: Int.ltu Int.zero r = true)
+    (CASTED1: val_casted (Vint k) type_int32s)
+    (CASTED1: val_casted (Vint r) type_int32u),
+    hash_pre_cond_args r [Vint k; Vint r].
+
+Inductive hash_post_cond_retv range : Values.val -> Prop :=
+| hash_post_cond_retv_intro: forall r    
+    (INRAN: Int.ltu r range = true),
+    hash_post_cond_retv range (Vint r).
+
+(** Pre/Post-conditions parameterized by the function name *)
+Definition linked_list_args_pre_conds r (f: ident) : list Values.val -> Prop :=
+  if ident_eq f hash then
+    hash_pre_cond_args r
+  else fun _ => True.
+
+Definition linked_list_retv_post_conds r (f: ident) : Values.val -> Prop :=
+  if ident_eq f hash then
+    hash_post_cond_retv r
+  else fun _ => True.
+
+Definition length_of_args (f: ident) : nat :=
+  if ident_eq f find then
+    2
+  else
+    if ident_eq f hash then
+      2     
+  else O.
+
+(* Initial preservation and progress *)
+Inductive vq_hash_map (w: hmap_world) : rust_query -> Prop :=
+(* incoming call of linked_list (i.e., the outgoing call of hmap) *)
+| vq_hash_map_intro1: forall b f targs tres tcc vargs m orgs rels fid
+    (FINDF: Genv.find_funct_ptr (globalenv w.(hmap_senv) linked_list_mod) b = Some (Internal f))
+    (NFHMAP: Genv.is_internal (Genv.globalenv w.(hmap_senv) hash_map_prog) (Vptr b Ptrofs.zero) = false)
+    (TYF: type_of_function f = Tfunction orgs rels targs tres tcc)
+    (NOTDROP: fn_drop_glue f = None)
+    (CASTED: val_casted_list vargs targs)
+    (SUP: Mem.sup_include (Genv.genv_sup w.(hmap_senv)) (Mem.support m))
+    (SYM: Genv.invert_symbol w.(hmap_senv) b = Some fid)
+    (PRECOND: linked_list_args_pre_conds w.(hmap_hash_range) fid vargs)
+    (FIDEQ: w.(hmap_callee) = inl fid)
+    (LEN: length_of_args fid = length vargs),
+    vq_hash_map w (rsq (Vptr b Ptrofs.zero) (mksignature orgs rels (type_list_of_typelist targs) tres tcc (globalenv w.(hmap_senv) linked_list_mod)) vargs m)
+(* outgoing call (which is specific to the definition of the C
+module..). For now, we only support calling the process function from
+Rust side. Other functions in the C module are static. *)
+| vq_hash_map_intro2: forall b f targs tres tcc vargs m orgs rels fid
+    (FINDF: Genv.find_funct_ptr (Genv.globalenv w.(hmap_senv) hash_map_prog) b = Some (Ctypes.Internal f))
+    (NFLINK: Genv.is_internal (globalenv w.(hmap_senv) linked_list_mod) (Vptr b Ptrofs.zero)= false)
+    (TYF: Clight.type_of_function f = Ctypes.Tfunction (to_ctypelist targs) (to_ctype tres) tcc)
+    (CASTED: val_casted_list vargs targs)
+    (SUP: Mem.sup_include (Genv.genv_sup w.(hmap_senv)) (Mem.support m))
+    (SYM: Genv.invert_symbol w.(hmap_senv) b = Some fid)
+    (** we only permit process function be called from Rust *)
+    (ONLYPROCESS: fid = process)
+    (PRECOND: linked_list_args_pre_conds w.(hmap_hash_range) fid vargs)
+    (FIDEQ: w.(hmap_callee) = inr fid)
+    (LEN: length_of_args fid = length vargs),
+    vq_hash_map w (rsq (Vptr b Ptrofs.zero) (mksignature orgs rels (type_list_of_typelist targs) tres tcc (globalenv w.(hmap_senv) linked_list_mod)) vargs m).
+    
+Inductive vr_hash_map (w: hmap_world) : rust_reply -> Prop :=
+(* return from linked_list module *)
+| vr_hash_map_intro1: forall v m fid
+    (FIDEQ: w.(hmap_callee) = inl fid)
+    (POSTCOND: linked_list_retv_post_conds w.(hmap_hash_range) fid v),
+    vr_hash_map w (rsr v m).
+
